Fix

Cslib/Computability/Machines/MultiTapeTuring/ListEncoding.lean
@@ -108,6 +108,14 @@ public def MultiTapeTM.eval_list
   (tm.eval (listToTape ∘ tapes)).bind fun tapes => tapesToLists tapes
 
 @[simp]
+public def MultiTapeTM.HaltsOnLists_of_evalList_eq_some
+    (tm : MultiTapeTM k (WithSep Symbol))
+    (tapes : Fin k → List (List Symbol))
+    (h_eval : (tm.eval_list tapes).Dom) :
+  tm.HaltsOnLists tapes := by
+  sorry
+
+@[simp]
 public theorem MultiTapeTM.HaltsOnLists_of_eval_list
     {tm : MultiTapeTM k (WithSep Symbol)}
     {tapes : Fin k → List (List Symbol)}
@@ -132,6 +140,15 @@ public def MultiTapeTM.eval_list_tot
     (tapes : Fin k → List (List Symbol)) :
   Fin k → List (List Symbol) :=
     (tm.eval_list tapes).get (tm.eval_list_dom_of_halts_on_lists (h_alwaysHalts tapes))
+
+@[simp]
+public lemma MultiTapeTM.eval_list_tot_eq
+    (tm : MultiTapeTM k (WithSep Symbol))
+    (h_alwaysHalts : ∀ tapes, tm.HaltsOnLists tapes)
+    (tapes : Fin k → List (List Symbol)) :
+  (tm.eval_list_tot) h_alwaysHalts tapes =
+    (tm.eval_list tapes).get (tm.eval_list_dom_of_halts_on_lists (h_alwaysHalts tapes)) := by
+  simp
 
 @[simp, grind =]
 public theorem MultiTapeTM.extend_eval_list
@@ -201,8 +218,8 @@ for an empty initial tape or the rightmost non-blank cell. -/
 -- TODO we could even make this Part now.
 public def MultiTapeTM.spaceUsed_list
     (tm : MultiTapeTM k (WithSep Symbol))
-    (tapes : Fin k → List (List Symbol))
-    (h_halts : ∀ tapes, tm.HaltsOn tapes := by simp) : Fin k → ℕ := sorry
+    (h_halts : ∀ tapes, tm.HaltsOnLists tapes := by simp)
+    (tapes : Fin k → List (List Symbol)) : Fin k → ℕ := sorry
 
 /-- The space initially used by a Turing machine that has the given tape configuration. -/
 public def spaceUsed_init (tapes : Fin k → List (List Symbol)) : Fin k → ℕ := fun i =>
@@ -212,11 +229,12 @@ public def spaceUsed_init_simp (tapes : Fin k → List (List Symbol)) (i : Fin k
   spaceUsed_init tapes i = (listToString (tapes i)).length := by simp [spaceUsed_init]
 
 @[simp]
-public lemma spaceUsed_init_le_spaceUsed {k : ℕ} {Symbol : Type}
+public lemma spaceUsed_init_le_spaceUsed
   {tm : MultiTapeTM k (WithSep Symbol)}
+  (h_halts : ∀ tapes, tm.HaltsOnLists tapes := by simp)
   (tapes : Fin k → List (List Symbol))
   (i : Fin k) :
-  spaceUsed_init tapes i ≤ MultiTapeTM.spaceUsed_list tm tapes sorry i := by
+  spaceUsed_init tapes i ≤ MultiTapeTM.spaceUsed_list tm h_halts tapes i := by
   sorry
 
 -- TODO for machines running on lists, we can actually have more precise head stats:
