Cslib/Computability/Machines/MultiTapeTuring/IsZeroRoutine.lean
@@ -33,24 +33,13 @@ public theorem isZero_eval_list {i : Fin k} {tapes : Fin k → List (List OneTwo
 
 @[simp]
 public theorem isZero_spaceUsed_list {i j : Fin k} {tapes : Fin k → List (List OneTwo)} :
-  (isZero i).spaceUsed_list tapes (by simp [isZero]) = Function.update (spaceUsed_init tapes) i
+  (isZero i).spaceUsed_list (by simp [isZero]) tapes = Function.update (spaceUsed_init tapes) i
     (if (tapes i).headD [] = [] then
       (listToString ([OneTwo.one] :: (tapes i).tail)).length
     else
       (listToString (tapes i)).length) := by
-  simp only [isZero, ite_spaceUsed_list]
-  by_cases h : j = i
-  · simp only [List.headD_eq_head?_getD, pop_halts, implies_true, push_halts_on,
-    MultiTapeTM.seq_spaceUsed_list, pop_spaceUsed, pop_eval_list, Part.get_some,
-    push_spaceUsed_list, Function.update_self, listToString_length_cons, List.length_cons,
-    List.length_nil, zero_add, Nat.reduceAdd]
-    sorry
-    -- cases (tapes i) with
-    -- | nil =>  grind
-    -- | cons hd tl => grind
-  · simp [h]
-    -- grind
-    sorry
+  simp [isZero, spaceUsed_init_simp]
+  sorry
 
 
 end Routines
