Cslib/Computability/Machines/MultiTapeTuring/PopRoutine.lean
@@ -28,11 +28,8 @@ lemma pop₁_eval_list {tapes : Fin 1 → List (List α)} :
   sorry
 
 @[simp]
-lemma pop₁_halts_on : ∀ tapes, (pop₁ (α := α)).haltsOn tapes := by sorry
-
-@[simp]
 lemma pop₁_spaceUsed_list {tapes : Fin 1 → List (List α)} :
-    (pop₁ (α := α)).spaceUsed_list tapes = spaceUsed_init tapes := by
+    (pop₁ (α := α)).spaceUsed_list (by simp) tapes = spaceUsed_init tapes := by
   sorry
 
 /--
@@ -49,12 +46,8 @@ public theorem pop_eval_list {k : ℕ} {i : Fin k}
   simp_all [pop]
 
 @[simp]
-public theorem pop_halts {k : ℕ} {i : Fin k} : ∀ tapes, (pop i (α := α)).haltsOn tapes := by
-  simp [pop]
-
-@[simp]
 public theorem pop_spaceUsed {k : ℕ} {i : Fin k} {tapes : Fin k → List (List α)} :
-  (pop i).spaceUsed_list tapes (h_halts := pop_halts) = spaceUsed_init tapes := by
+  (pop i).spaceUsed_list (by simp) tapes = spaceUsed_init tapes := by
   have h_inj : [i].get.Injective := by intro x y; grind
   sorry
 
