Cslib/Computability/Machines/MultiTapeTuring/PushRoutine.lean
@@ -29,7 +29,7 @@ lemma push₁_eval_list {w : List α} {tapes : Fin 1 → List (List α)} :
 
 @[simp]
 lemma push₁_spaceUsed_list {w : List α} {tapes : Fin 1 → List (List α)} {i : Fin 1} :
-    (push₁ w).spaceUsed_list tapes sorry i = (listToString (w :: (tapes 0))).length := by
+    (push₁ w).spaceUsed_list (by simp) tapes i = (listToString (w :: (tapes 0))).length := by
   sorry
 
 /--
@@ -47,15 +47,9 @@ public theorem push_eval_list {k : ℕ}
   simp_all [push]
 
 @[simp]
-public theorem push_halts_on {k : ℕ} {i : Fin k} {w : List α} :
-  ∀ tapes, (push i w).haltsOn tapes := by
-  sorry
-
-
-@[simp]
 public theorem push_spaceUsed_list {k : ℕ} {i : Fin k} {w : List α}
   {tapes : Fin k → List (List α)} :
-    (push i w).spaceUsed_list tapes = Function.update (spaceUsed_init tapes)
+    (push i w).spaceUsed_list (by simp) tapes = Function.update (spaceUsed_init tapes)
       i (listToString (w :: (tapes i))).length := by
   simp [push]
   sorry
